\documentclass{article}
\usepackage{amsmath}
\usepackage{listings}
\usepackage{xcolor}
\usepackage{amsfonts}
\usepackage{amsthm}
\usepackage{amssymb}
\usepackage{geometry}
\geometry{left=2.0cm,right=2.0cm,top=2.5cm,bottom=2.5cm}
\newtheoremstyle{break}%
    {}{}%
    {\itshape}{}%
    {\bfseries}{}% % Note that final punctuation is omitted.
    {\newline}{}
\theoremstyle{break}
\newtheorem*{definition}{Definition}
\newtheorem*{proof_break}{Proof.}
\lstset{
    numbers=left, 
    numberstyle= \tiny, 
    keywordstyle= \color{ blue!70},
    commentstyle= \color{red!50!green!50!blue!50}, 
    frame=shadowbox, % 阴影效果
    rulesepcolor= \color{ red!20!green!20!blue!20} ,
    escapeinside=``, % 英文分号中可写入中文
    xleftmargin=2em,xrightmargin=2em, aboveskip=1em,
    framexleftmargin=2em
} 

\begin{document}
    \title{HW2}
    \author{Sitian Qian 1600011388}
    \maketitle

    \section{Problem 1}
    \subsection{Subproblem 1}
    \begin{proof_break}\par
        Firstly we can write $\hat{\sigma}_a^2$ and $\hat{\sigma}_b^2$ as following:
        $$\left[\begin{array}{c}{\hat{\sigma}_{a}^{2}} \\ {\hat{\sigma}_{b}^{2}}\end{array}\right]=\frac{1}{nq} \sum_{k=1}^{n}\left[\begin{array}{c}{\sum_{j=1}^{q}(\varepsilon_{q(k-1)+j}^2)} \\ {(\sum_{j=1}^{q}\varepsilon_{q(k-1)+j})^{2}}\end{array}\right]$$
        Since $\{\varepsilon_{qk}\}$ is an iid sequence, $\{\sum_{j=1}^{q}(\varepsilon_{q(k-1)+j}^2)\}$,$\{(\sum_{j=1}^{q}\varepsilon_{q(k-1)+j})^{2}\}$ are also iid sequences. Which enables us to use central limit theorem to obtain the
        asymptotic distribution.\newline
        The expectation is easy to obtain: 
        $$\mathbb{E}\left[\begin{array}{c}{\sum_{j=1}^{q}(\varepsilon_{q(k-1)+j}^2)} \\ {(\sum_{j=1}^{q}\varepsilon_{q(k-1)+j})^{2}}\end{array}\right]=\left[\begin{array}{l}{q \sigma^{2}} \\ {q \sigma^{2}}\end{array}\right]$$
        The variance can be obtained as below: 
        \begin{align*}
            &Var(\sum_{j=1}^{q}(\varepsilon_{q(k-1)+j}^2))\\
            =&\sum_{j=1}^q(Var(\varepsilon^2_{q(k-1)+j}))\\
            =&q(A-1)\sigma^4
        \end{align*}
        (Here I use $A$ to represent $\mathbb{E}{x}^4$, x is subject to standard normal distribution, in fact $A=3$;)
        \begin{align*}
            &Var((\sum_{j=1}^{q}\varepsilon_{q(k-1)+j})^2)\\
            =&qA\sigma^4+6*C_q^2\sigma^4-q^2*\sigma^4\\
            =&(Aq+2q^2-3q)\sigma^4
        \end{align*}
        and
        \begin{align*}
            &Cov((\sum_{j=1}^{q}\varepsilon_{q(k-1)+j})^2,\sum_{j=1}^{q}(\varepsilon_{q(k-1)+j}^2))\\
            =&Var(\sum_{j=1}^{q}(\varepsilon_{q(k-1)+j}^2))+Cov(\sum_{i=1}^{q}\sum_{j\neq{i},j=1}^{q}(\varepsilon_{q(k-1)+i}\varepsilon_{q(k-1)+j}),\sum_{j=1}^{q}(\varepsilon_{q(k-1)+j}^2))\\
            =&q(A-1)\sigma^4
        \end{align*}
        Finally we get:
        \begin{align*}
        Var\left(\left[\begin{array}{c}{\sum_{j=1}^{q}(\varepsilon_{q(k-1)+j}^2)} \\ {(\sum_{j=1}^{q}\varepsilon_{q(k-1)+j})^2}\end{array}\right]\right)=\left[\begin{array}{cc}{2q\sigma^4} & {2q\sigma^4}\\ {2q\sigma^{4}} & {2q^2\sigma^{4}}\end{array}\right]
        \end{align*}
        Therefore, using CLT,
            $$\sqrt{n}\left(\left[\begin{array}{c}{\hat{\sigma}_{a}^{2}} \\ {\hat{\sigma}_{b}^{2}}\end{array}\right]-\left[\begin{array}{c}{\sigma^{2}} \\ {\sigma^{2}}\end{array}\right]\right) \rightarrow_{d} \mathbb{N}\left(0,\left[\begin{array}{cc}{\frac{2\sigma^{4}}{q}} & {\frac{2\sigma^4}{q}} \\ {\frac{2\sigma^{4}}{q}} & {2\sigma^4}\end{array}\right]\right)$$
        With the Delta method, representing $J_r=\frac{\hat{\sigma}_b^2}{\hat{\sigma}_a^2}-1$ by $J_{r}=h(\hat{\sigma}_{a}^{2}, \hat{\sigma}_{b}^{2})$,we have: 
        $$\sqrt{n}(h(\hat{\beta})-h(\beta)) \rightarrow_{d} \mathbb{N}\left(0, \nabla h^{T}(\beta) D \nabla h(\beta)\right.$$
        where $\hat{\beta}=(\hat{\sigma}_{a}^{2}, \hat{\sigma}_{b}^{2})^{T}$, $\beta=\vec{0}$, and $D=\left[\begin{array}{cc}{\frac{2\sigma^{4}}{q}} & {\frac{2\sigma^4}{q}} \\ {\frac{2\sigma^{4}}{q}} & {2\sigma^4}\end{array}\right]$,
        \newline
        Namely, the distribution of $J_r$ is,
        $$\sqrt{n}\left(J_{r}-0\right) \rightarrow_{d} \mathbb{N}\left(0,\left[\begin{array}{cc}{-\frac{1}{\sigma^{2}}} & {\frac{1}{\sigma^{2}}}\end{array}\right]\left[\begin{array}{cc}{\frac{A-\sigma^{4}}{2}} & {\frac{A-\sigma^{4}}{2}} \\ {\frac{A-\sigma^{4}}{2}} & {\frac{A+\sigma^{4}}{2}}\end{array}\right]\left[\begin{array}{c}{-\frac{1}{\sigma^{2}}} \\ {\frac{1}{\sigma^{2}}}\end{array}\right]\right)=\mathbb{N}(0,1)$$
    \end{proof_break}
    
\end{document}